Some refactoring of ST2 related files + updating  to new All effect library

examples/relational/ro.fst
@@ -1,7 +1,7 @@
 (*--build-config
-    options:--admit_fsi Set;
+    options:--admit_fsi Set --z3timeout 300;
     variables:LIB=../../lib;
-    other-files:$LIB/ext.fst $LIB/set.fsi $LIB/heap.fst $LIB/st.fst $LIB/st2.fst $LIB/bytes.fst $LIB/list.fst
+    other-files:$LIB/set.fsi $LIB/heap.fst $LIB/st.fst $LIB/all.fst $LIB/st2.fst $LIB/bytes.fst $LIB/list.fst sample.fst xor.fst
   --*)
 
 module Ro
@@ -10,22 +10,30 @@ open Comp
 open Heap
 open List
 open Bytes
+open Xor
+open Bijection
+open Sample
 
 type map (a:Type) (b:Type) = list (a * b)
 
-let eta = 16
+type key = bytes
+type tag = block
 
-type key = b:bytes
-type tag = b:bytes{length(b)=eta}
-
-(* TODO? *)
 (* an abstract relational predicate on correctly-generated entries *)
-assume logic type safe_key (k0:key) (k1:key)
-let safe_key_unique = assume (forall k0 k1 k1'.
+opaque type safe_key (k0:key) (k1:key) = (exists (f:bij #key #key). k1 = f k0)
+(*  type safe_key (k0:key) (k1:key) = k0 = k1 *)
+assume Safe_key_unique  : (forall k0 k1 k1'.
+                               {:pattern (safe_key k0 k1); (safe_key k0 k1')}
                                (safe_key k0 k1 /\ safe_key k0 k1' ==> k1 = k1'))
-let safe_key_unique' = assume (forall k0 k0' k1.
+assume Safe_key_unique  : (forall k0 k0' k1.
+                               {:pattern (safe_key k0 k1); (safe_key k0' k1)}
                                (safe_key k0 k1 /\ safe_key k0' k1 ==> k0 = k0'))
-assume logic type safe (k0:key) (k1:key) (t0:tag) (t1:tag)
+opaque type safe (t0:tag) (t1:tag) = (exists (f:bij #tag #tag). t1 = f t0)
+
+ val bij2safe : f:bij #tag #tag -> t0:tag -> t1:tag ->
+               Lemma (requires (t1 = f t0))
+                     (ensures  (safe t0 t1))
+let bij2safe f t0 t1 = ()
 
 type alloc =
   | Hon: alloc
@@ -40,7 +48,7 @@ type state_hash =
 
 type Ok : log -> log -> Type =
   | Null: Ok [] []
-  | ConsH: k0:key -> k1:key{safe_key k0 k1} -> t0:tag -> t1:tag{safe k0 k1 t0 t1}
+  | ConsH: k0:key -> k1:key{safe_key k0 k1} -> t0:tag -> t1:tag{safe t0 t1}
            -> log0:log{is_None (assoc k0 log0)}
            -> log1:log{is_None (assoc k1 log1)}
            -> p: Ok log0 log1
@@ -51,11 +59,13 @@ type Ok : log -> log -> Type =
            -> p: Ok log0 log1
            -> Ok ((k ,(Adv,t ))::log0) ((k, (Adv,t ))::log1)
 
-assume val ok_as_proof : l0:log -> l1:log {Ok l0 l1} -> Tot (Ok l0 l1)
-assume val ok_as_refinement : #l0:log -> #l1:log  -> p:Ok l0 l1 -> Tot (u:unit{Ok l0 l1})
+type fresh_keys (k0:key) (k1:key) (l0:log) (l1:log) = is_None (assoc k0 l0) /\ is_None (assoc k1 l1)
 
-val ok_consH : k0:key -> k1:key{safe_key k0 k1} -> t0:tag
-              -> t1:tag{safe k0 k1 t0 t1}
+assume val ok_as_refinement : #l0:log -> #l1:log  -> p:Ok l0 l1 -> Tot (u:unit{Ok l0 l1})
+assume val ok_as_proof : l0:log -> l1:log{Ok l0 l1} -> Tot (Ok l0 l1)
+
+ val ok_consH : k0:key -> k1:key{safe_key k0 k1} -> t0:tag
+              -> t1:tag{safe t0 t1}
               -> l0:log{is_None (assoc k0 l0)}
               -> l1:log{is_None (assoc k1 l1) /\ Ok l0 l1} ->
                Lemma (requires True)
@@ -63,14 +73,14 @@ val ok_consH : k0:key -> k1:key{safe_key k0 k1} -> t0:tag
                      [SMTPat (assoc k0 l0);SMTPat (assoc k1 l1)]
 let ok_consH k0 k1 t0 t1 l0 l1 = ok_as_refinement(ConsH k0 k1 t0 t1 l0 l1 (ok_as_proof l0 l1))
 
-val ok_consA : k:key -> t:tag -> l0:log{is_None(assoc k l0)}
+ val ok_consA : k:key -> t:tag -> l0:log{is_None(assoc k l0)}
                -> l1:log{is_None(assoc k l1) /\ Ok l0 l1}
                -> Lemma (requires True)
                         (ensures Ok ((k,(Adv,t))::l0) ((k,(Adv,t))::l1))
                         [SMTPat (assoc k l0);SMTPat (assoc k l1)]
 let ok_consA k t l0 l1 = ok_as_refinement (ConsA k t l0 l1 (ok_as_proof l0 l1))
 
-val ok_adv_eq' : l0:log -> l1:log -> p:Ok l0 l1 -> k:key
+ val ok_adv_eq' : l0:log -> l1:log -> p:Ok l0 l1 -> k:key
                 -> Lemma
                    (requires True)
                    (ensures (forall t. assoc k l0 = Some(Adv, t) <==>
@@ -81,7 +91,7 @@ let rec ok_adv_eq' l0 l1 p k = match p with
         | ConsA _ _ tl0 tl1 p' -> ok_adv_eq' tl0 tl1 p' k
 
 
-val ok_adv_eq : l0:log -> l1:log{Ok l0 l1} ->  k:key
+ val ok_adv_eq : l0:log -> l1:log{Ok l0 l1} ->  k:key
                 -> Lemma
                    (requires True)
                    (ensures (forall t. assoc k l0 = Some(Adv, t) <==>
@@ -90,7 +100,7 @@ val ok_adv_eq : l0:log -> l1:log{Ok l0 l1} ->  k:key
 let ok_adv_eq l0 l1 k = ok_adv_eq' l0 l1 (ok_as_proof l0 l1) k
 
 
-val ok_hon_safe' : k0:key -> k1:key -> l0:log -> l1:log -> p:Ok l0 l1
+ val ok_hon_safe' : k0:key -> k1:key -> l0:log -> l1:log -> p:Ok l0 l1
                 -> Lemma
                    (requires (safe_key k0 k1))
                    (ensures ( (is_Some(assoc k0 l0) /\ is_Hon(fst (Some.v(assoc k0 l0)))) <==>
@@ -109,13 +119,13 @@ val ok_hon_safe: k0:key -> k1:key -> l0:log -> l1:log {p:Ok l0 l1}
 let ok_hon_safe k0 k1 l0 l1 = ok_hon_safe' k0 k1 l0 l1 (ok_as_proof l0 l1)
 
 
-val ok_hon_safe2' : k0:key -> k1:key -> l0:log -> l1:log -> p:Ok l0 l1
+ val ok_hon_safe2' : k0:key -> k1:key -> l0:log -> l1:log -> p:Ok l0 l1
                 -> Lemma
                    (requires (safe_key k0 k1))
                    (ensures (is_Some(assoc k0 l0) /\ is_Some(assoc k1 l1) /\
                              is_Hon(fst(Some.v (assoc k0 l0))) /\
                              is_Hon(fst(Some.v (assoc k0 l0))) ==>
-                               safe k0 k1 (snd(Some.v (assoc k0 l0))) (snd(Some.v (assoc k1 l1)))))
+                               safe (snd(Some.v (assoc k0 l0))) (snd(Some.v (assoc k1 l1)))))
 let rec ok_hon_safe2' k0 k1 l0 l1 p = match p with
         | Null -> ()
         | ConsH k0' k1' t01 t1' tl0 tl1 p' -> ok_hon_safe2' k0 k1 tl0 tl1 p'
@@ -128,23 +138,13 @@ val ok_hon_safe2 : k0:key -> k1:key -> l0:log -> l1:log{Ok l0 l1}
                     (ensures (is_Some(assoc k0 l0) /\ is_Some(assoc k1 l1) /\
                               is_Hon(fst(Some.v (assoc k0 l0))) /\
                               is_Hon(fst(Some.v (assoc k0 l0))) ==>
-                                safe k0 k1 (snd(Some.v (assoc k0 l0))) (snd(Some.v (assoc k1 l1)))))
+                                safe (snd(Some.v (assoc k0 l0))) (snd(Some.v (assoc k1 l1)))))
                                 [SMTPat (assoc k0 l0); SMTPat (assoc k1 l1)]
 let ok_hon_safe2 k0 k1 l0 l1 = ok_hon_safe2' k0 k1 l0 l1 (ok_as_proof l0 l1)
-
 type goodstate_hash (s1:state_hash) (s2:state_hash) =
             s1.bad = true \/ s2.bad = true \/ Ok s1.l s2.l
 
 assume val s : ref state_hash
-
-assume val sample_hon : k0:key -> k1:key ->
-                 ST2 (tag * tag)
-                   (requires (fun _ -> True))
-                   (ensures (fun h2' p h2 -> h2' = h2 /\ safe k0 k1 (fst p) (snd p)))
-assume val sample_adv : unit ->
-                 ST2 (tag * tag)
-                   (requires (fun _ -> True))
-                   (ensures (fun h2' p h2 -> h2' = h2 /\ fst p = snd p))
 
 (* Actual non-relational code of hash_hon : *)
 (*
@@ -157,27 +157,33 @@ let hash_hon k = match assoc k (!s),l with
 *)
 
 
-val hash_hon:  k0:key -> k1:key ->
+opaque val hash_hon:  k0:key -> k1:key -> f:bij #tag #tag ->
                ST2 (option tag * option tag)
                (requires (fun h2 -> goodstate_hash (sel (fst h2) s) (sel (snd h2) s) /\
                           safe_key k0 k1))
-               (ensures (fun _ p h2 -> (sel (fst h2) s).bad \/
+               (ensures (fun h2' p h2 -> (sel (fst h2) s).bad \/
                                        (sel (snd h2) s).bad \/
                                        (is_Some (fst p) /\ is_Some (snd p) /\
-                                          safe k0 k1 (Some.v(fst p)) (Some.v(snd p))
+                                          safe (Some.v(fst p)) (Some.v(snd p))
+                                          /\ (fresh_keys k0 k1 ((sel (fst h2') s).l) ((sel (snd h2') s).l)
+                                              ==> Some.v (snd p) = f (Some.v (fst p)))
                                           /\ Ok (sel (fst h2) s).l (sel (snd h2) s).l)))
 
-val hash_hon2: k0:key -> k1:key ->
+                                  (* Why does (f:bij #tag #tag) not work here?*)
+opaque val hash_hon2: k0:key -> k1:key -> f:(tag -> Tot tag){bijection f} ->
                ST2 (option tag * option tag)
                (requires (fun h2 -> goodstate_hash (sel (fst h2) s) (sel (snd h2) s) /\
                           safe_key k0 k1))
-               (ensures (fun _ p h2 -> (sel (fst h2) s).bad \/
+               (ensures (fun h2' p h2 -> (sel (fst h2) s).bad \/
                                        (sel (snd h2) s).bad \/
                                        (is_Some (fst p) /\ is_Some (snd p) /\
-                                          safe k0 k1 (Some.v(fst p)) (Some.v(snd p))
+                                          safe (Some.v(fst p)) (Some.v(snd p))
+                                          /\ (fresh_keys k0 k1 ((sel (fst h2') s).l) ((sel (snd h2') s).l)
+                                              ==> Some.v (snd p) = f (Some.v (fst p)))
                                           /\ Ok (sel (fst h2) s).l (sel (snd h2) s).l)))
 
-val hash_adv:  k:key ->
+
+opaque val hash_adv:  k:key ->
                ST2 (option tag * option tag)
                (requires (fun h2 -> goodstate_hash (sel (fst h2) s) (sel (snd h2) s)))
                (ensures (fun _ p h2 -> (sel (fst h2) s).bad \/
@@ -199,7 +205,7 @@ let hash_hon' k r = match assoc k (!s).l with
                     s := {bad = (!s).bad; l= (k,(Hon,t))::(!s).l} ;
                     add_some t
 
-let hash_hon k0 k1  = let r0, r1 = sample_hon k0 k1 in
+let hash_hon k0 k1 f = let r0, r1 = sample f in
                       (compose2 (fun k -> hash_hon' k r0)
                                 (fun k -> hash_hon' k r1)
                                 k0 k1)
@@ -209,8 +215,9 @@ let case_Adv  _     = s:={bad = true; l=(!s).l}; None
 let case_None (k,t) = s:={bad = (!s).bad; l = (k,(Hon,t))::(!s).l}; add_some t
 
 assume val sample_single : unit -> Tot tag
+#reset-options
 
-let hash_hon2 k0 k1 =
+let hash_hon2 k0 k1 f =
   let l0, l1 = compose2 (fun _ -> (!s).l) (fun _ -> (!s).l) () () in
   match assoc k0 l0, assoc k1 l1 with
   | Some (Hon,t0), Some (Hon,t1) -> compose2 (fun x -> case_Hon x) (fun x -> case_Hon x) t0 t1
@@ -225,7 +232,7 @@ let hash_hon2 k0 k1 =
                                     compose2 (fun x -> case_None x) (fun x -> case_Hon x) (k0,t0) t1
   | None         , Some (Adv,t1) -> let t0 = sample_single () in
                                     compose2 (fun x -> case_None x) (fun x -> case_Adv x) (k0,t0) ()
-  | None         , None          -> let t0, t1 = sample_hon k0 k1 in
+  | None         , None          -> let t0, t1 = sample f in
                                     compose2 (fun x -> case_None x) (fun x -> case_None x) (k0,t0) (k1,t1)
 
 let hash_adv' k r =  match assoc k (!s).l with
@@ -236,65 +243,82 @@ let hash_adv' k r =  match assoc k (!s).l with
                     add_some t
 
 
-let hash_adv k  = let r0, r1 = sample_adv () in
+let hash_adv k  = let r0, r1 = sample (fun x->x) in
                   compose2 (fun k -> hash_adv' k r0)
                            (fun k -> hash_adv' k r1)
                            k k
 
+
 (* Simple Encryption Scheme based on ro *)
+module Encryption
 
-type injection (#a:Type) (f:a -> Tot a) = (forall x y. f x = f y ==> x = y)
-type surjection (#a:Type) (f:a -> Tot a) = (forall y. (exists x. f x = y))
-type bijection (#a:Type) (f:a -> Tot a) = injection f /\ surjection f
+open Comp
+open Heap
+open Bijection
+open Sample
+open Xor
+open Bytes
+open List
+open Ro
 
-assume val sample : #a:Type
-                    -> f:(a -> Tot a){bijection f}
-                    -> ST2 (a * a)
-                       (requires (fun _ -> True))
-                       (ensures (fun h2' p  h2 -> h2' = h2 /\ fst p = f (snd p)))
 
 assume val append : bytes -> bytes -> Tot bytes
-
-type block = b:bytes{length(b)=eta}
-
-assume val xor : block -> block -> Tot block
-
-let xor_sym = assume(forall a b. xor a b = xor b a)
-let xor_inv = assume(forall a b. xor (xor a b) a = b)
-let xor_ass = assume(forall a b c. xor (xor a b) c = xor a (xor b c))
-val xor_inj : a:block -> b:block -> c:block
-              -> Lemma
-              (requires (xor a b = xor a c))
-              (ensures (b = c))
-              [SMTPat (xor a b = xor a c)]
-let xor_inj a b c = cut (b2t (xor (xor a b) a = xor (xor a c) a))
 
 val encrypt : block -> block -> Tot block
 let encrypt p k = xor p k
 val decrypt : block -> block -> Tot block
 let decrypt c k = xor c k
 
+(*
 type state_enc =
   { bad': bool; (* set iff a nonce was sampled twice *)
     l':log }    (* the log keeps track of returned nonces *)
+*)
 
-type good_state_enc (s:state_enc) = s.bad' = false
-(*
+(* type good_state_enc (s:state_enc) = s.bad' = false *)
 
-val encrypt_hon : k0:bytes ->  k1:bytes -> p0:block -> p1:block ->
-              ST2 (option(block * block) * option(block * block))
+opaque type safe_key_pre (k0:bytes) (k1:bytes) = (forall (r:block). safe_key (append k0 r) (append k1 r))
+
+val lemma_safe_key_pre : k0:bytes -> k1:bytes{safe_key_pre k0 k1} -> r0:block -> r1:block{r0=r1}
+                         -> Lemma (safe_key (append k0 r0) (append k1 r1))
+let lemma_safe_key_pre k0 k1 r0 r1 = ()
+
+type mp : Type =
+  | MkMP : a:block -> b:block -> mp
+
+
+#reset-options
+
+val xor_inverse_lemma : a:block -> Lemma (bijection #block #block (fun x -> xor a x))
+let xor_inverse_lemma a = ()
+
+
+#reset-options
+
+val encrypt_hon : k0:bytes ->  k1:bytes{safe_key_pre k0 k1}
+                  -> p0:block-> p1:block ->
+                  ST2 (option mp * option mp)
                   (requires (fun h2 -> goodstate_hash (sel (fst h2) s) (sel (snd h2) s)))
                   (ensures  (fun h2' p h2 -> (sel (fst h2) s).bad  \/
                                              (sel (snd h2) s).bad  \/
                                              Ok (sel (fst h2) s).l (sel (snd h2) s).l /\
-                                             is_Some (fst p) /\ is_Some (snd p) /\
-                                             fst p = snd p))
-*)
-
+                                             is_Some (fst p) /\ is_Some (snd p)))
 (*
-let encrypt_hon k0 k1 p0 p1 = let r0, r1 = sample (fun x ->  x) in
-                  let h0, h1 = hash_hon (append k0 r0) (append k1 r1) in
-                  compose2 (fun (p,h,r) -> if is_Some h then Some ((encrypt p (Some.v h)),r) else None)
-                           (fun (p,h,r) -> if is_Some h then Some ((encrypt p (Some.v h)),r) else None)
-                           (p0, h0, r0) (p1, h1, r1)
+                                             (fresh_keys (append k0 (MkMP.a(Some.v (fst p))))
+                                                         (append k1 (MkMP.a(Some.v (snd p))))
+                                                         (sel (fst h2') s).l
+                                                         (sel (snd h2') s).l ==>
+                                                  fst p = snd p)
 *)
+let encrypt_hon k0 k1 p0 p1 =
+                  let sample_fun = (fun x -> xor (xor p0 p1) x) in
+                  xor_inverse_lemma (xor p0 p1);
+                  cut(bijection #block #block sample_fun);
+                  let r0, r1 = sample (fun x ->  x) in
+                  let kh0, kh1 = append k0 r0, append k1 r1 in
+                  lemma_safe_key_pre k0 k1 r0 r1;
+                  cut (safe_key kh0 kh1);
+                  let h0, h1 = hash_hon kh0 kh1 (sample_fun)  in
+                  let a = if is_Some h0 then Some (MkMP (encrypt p0 (Some.v h0)) r0) else None in
+                  let b = if is_Some h1 then Some (MkMP (encrypt p1 (Some.v h1)) r1) else None in
+                  a,b
